crypto_examples/ntt_rec2.dfy
@@ -1,0 +1,172 @@
+include "ntt_rec.dfy"
+
+module ntt_rec2 {
+    import opened Seq
+    import opened Power
+    import opened Power2
+    import opened DivMod
+    import opened Mul
+    import opened pows_of_2
+    import opened omegas
+    import opened rindex
+    import opened ntt_rec
+
+    predicate poly_eval_chunks(ys: seq<seq<elem>>, clen: pow2_t)
+        requires 0 <= clen.exp <= L
+        requires |A()| == N == pow2(L).full
+    {
+        && |ys| == pow2_div(pow2(L), clen).full
+        && (forall ki: nat, i: nat | ki < |ys| && i < clen.full ::(
+            && |ys[ki]| == clen.full
+            && clen.full * ki + i >= 0
+            && ys[ki][i] == poly_eval(A(), omega_nk(clen, clen.full * ki + i))))
+    }
+
+    // lemma ntt_chunks_base_case(clen: pow2_t)
+    //     requires clen.exp == 0
+    //     ensures poly_eval_chunks(ys, len);
+
+    // lemma ntt_chunks_rec_case(ys': seq<seq<elem>>, k: nat,
+    //     ys: seq<seq<elem>>, clen: pow2_t)
+    //     requires 1 <= clen.exp <= L
+    //     requires k < |ys'| == pow2_div(pow2(L), clen).full
+    //     requires |ys'[k]| == clen.full;
+    //     requires poly_eval_chunks(ys, pow2_half(clen));
+    // {
+    //     assume |ys| == 2 * |ys'|;
+    //     var y_e := ys[2 * k];
+    //     var y_o := ys[2 * k + 1];
+    //     compute_y_ks(a: seq<elem>, 
+    //     a_e: seq<elem>, a_o: seq<elem>,
+    //     y_e, y_o,
+    //     len):
+    // }
+
+    // function method ntt_rec_chunk_combine()
+
+    // function method {:fuel 1} ntt_rec_chunks(clen: pow2_t): (ys: seq<seq<elem>>)
+    //     requires 0 <= clen.exp <= L
+    //     ensures poly_eval_chunks(ys, clen);
+    //     decreases clen.exp
+    // {
+    //     if clen.exp == 0 then
+    //         var ys := seq(N, i requires 0 <= i < N => [Ar()[i]]);
+    //         assume poly_eval_chunks(ys, clen);
+    //         ys
+    //     else
+    //         var ys := ntt_rec_chunks(pow2_half(clen));
+    //         var ccount := pow2_div(pow2(L), clen).full;
+    //         var ys' := seq(ccount, i requires 0 <= i < ccount => [0]);
+    //         assume false;
+    //         ys'
+    // }
+
+    function method ntt_rec2(a: seq<elem>, len: pow2_t, ghost idxs: seq<index_t>, ghost ki: nat) : (y: seq<elem>)
+        requires 2 <= len.full;
+        requires len.exp <= L;
+        requires |a| == |idxs| == len.full;
+        requires ki < pow2_div(pow2(L), len).full
+        requires ntt_indicies_inv(idxs, len, ki); 
+        ensures poly_eval_all_points(a, y, len);
+        ensures len.full == 2 ==> 
+            idxs[0].bins == Reverse(orignal_index(ki, 0, len).bins);
+        ensures len.full == 2 ==> 
+            idxs[1].bins == Reverse(orignal_index(ki, 1, len).bins);
+        decreases len.full
+    {
+        if len.full == 2 then 
+            var len' := pow2_half(len);
+            pow2_basics(len');
+
+            var a_e := even_indexed_terms(a, len');
+            var a_o := odd_indexed_terms(a, len');
+
+            assert a_e[0] == poly_eval(a_e, omega_nk(len', 0)) by {
+                assert a_e[0] == a[0];
+                ntt_rec_base_case(a_e, len');
+            }
+            assert a_o[0] == poly_eval(a_o, omega_nk(len', 0)) by {
+                assert a_o[0] == a[1];
+                ntt_rec_base_case(a_o, len');
+            }
+
+            var y_ks := compute_y_k(a, a_e, a_o, a_e, a_o, len, 0);
+            var y_k's := compute_y_k'(a, a_e, a_o, a_e, a_o, len, 0);
+
+            ntt_indicies_inv_consequence(idxs, len, ki);
+            [y_ks, y_k's]
+        else
+            var len' := pow2_half(len);
+            var a_e := even_indexed_terms(a, len');
+            var a_o := odd_indexed_terms(a, len');
+
+            ghost var idx_e := even_indexed_indices(idxs, len);
+            ghost var idx_o := odd_indexed_indices(idxs, len);
+
+            even_indexed_indices_reorder(idxs, len, idx_e, ki);
+            odd_indexed_indices_reorder(idxs, len, idx_o, ki);
+
+            var y_e := ntt_rec2(a_e, len', idx_e, 2 * ki);
+            var y_o := ntt_rec2(a_o, len', idx_o, 2 * ki + 1);
+
+            var y_ks := compute_y_ks(a, a_e, a_o, y_e, y_o, len);
+            var y_k's := compute_y_k's(a, a_e, a_o, y_e, y_o, len);
+            var y := y_ks + y_k's;
+
+            assert forall i: nat | i < len.full ::
+                y[i] == poly_eval(a, omega_nk(len, i)) by {
+                forall i: nat | i < len.full
+                    ensures y[i] == poly_eval(a, omega_nk(len, i))
+                {
+                    if i < len'.full {
+                        assert y[i] == y_ks[i];
+                    } else {
+                        var j := i - len'.full;
+                        assert y[i] == y_k's[j];
+                    }
+                }
+            }
+            y
+    }
+    function method A(): seq<elem>
+        ensures |A()| == N == pow2(L).full;
+
+    function method Ar(): seq<elem>
+        ensures |Ar()| == N == pow2(L).full;
+        ensures forall i | 0 <= i < N ::
+            Ar()[i] == A()[build_rev_index(i).v];
+
+    // function method {:fuel 1} build_level_chunks(len: pow2_t): (cs: seq<seq<elem>>)
+    //     requires 1 <= len.exp <= L
+    //     ensures |cs| == pow2_div(pow2(L), len).full;
+    //     ensures forall i | 0 <= i < |cs| :: |cs[i]| == len.full
+    //     decreases L - len.exp
+    // {
+    //     if len.exp == L then [A()]
+    //     else 
+    //         var a := build_level_chunks(pow2_double(len));
+    //         assert |a| == pow2(L - len.exp - 1).full by {
+    //             assert |a| == pow2(L).full / (pow2(len.exp + 1).full);
+    //             reveal Pow2();
+    //             assert len.exp + 1 <= L;
+    //             LemmaPowSubtracts(2, len.exp + 1, L);
+    //         }
+    //         assert |a| * 2 == pow2(L - len.exp).full by {
+    //             reveal Pow2();
+    //             LemmaPowAdds(2, L - len.exp - 1, 1);
+    //             LemmaPow1(2);
+    //         }
+    //         seq(|a| * 2, k requires 0 <= k < |a| * 2 => 
+    //             if k % 2 == 0 then even_indexed_terms(a[k/2], len)
+    //             else odd_indexed_terms(a[(k-1)/2], len))
+    // }
+
+    // function method get_level_chunk(len: pow2_t, ki: nat): (chunk: seq<elem>)
+    //     requires 1 <= len.exp <= L
+    //     requires ki < pow2_div(pow2(L), len).full;
+    //     ensures |chunk| == len.full
+    // {
+    //     build_level_chunks(len)[ki]
+    // }
+}
+
